cleanup: clean group context serialization in the keyschedule

fstar/test/MLS.Test.FromExt.KeySchedule.fst
@@ -17,7 +17,7 @@ let gen_epoch_output #cb group_id last_init_secret epoch inp =
   let commit_secret = hex_string_to_bytes inp.commit_secret in
   let psk_secret = hex_string_to_bytes inp.psk_secret in
 
-  let group_context = (ps_prefix_to_ps_whole ps_group_context_nt).serialize (gen_group_context (ciphersuite #bytes) (hex_string_to_bytes group_id) epoch (hex_string_to_bytes inp.tree_hash) (hex_string_to_bytes inp.confirmed_transcript_hash)) in
+  let group_context = gen_group_context (ciphersuite #bytes) (hex_string_to_bytes group_id) epoch (hex_string_to_bytes inp.tree_hash) (hex_string_to_bytes inp.confirmed_transcript_hash) in
   let last_init_secret = hex_string_to_bytes last_init_secret in
   let joiner_secret = extract_result (secret_init_to_joiner last_init_secret (Some commit_secret) group_context) in
   let welcome_secret = extract_result (secret_joiner_to_welcome_internal #bytes joiner_secret psk_secret) in
@@ -36,11 +36,11 @@ let gen_epoch_output #cb group_id last_init_secret epoch inp =
     if not (string_is_ascii inp.exporter_label && String.strlen inp.exporter_label < pow2 30 - 8) then
       failwith "gen_epoch_output: exporter label is not ascii"
     else
-      extract_result (mls_exporter exporter_secret inp.exporter_label (hex_string_to_bytes inp.exporter_context) (UInt32.v inp.exporter_length))
+      extract_result (mls_exporter (exporter_secret <: bytes) inp.exporter_label (hex_string_to_bytes inp.exporter_context) (UInt32.v inp.exporter_length))
   in
 
   {
-    group_context = bytes_to_hex_string group_context;
+    group_context = bytes_to_hex_string (serialize _ group_context);
     joiner_secret = bytes_to_hex_string joiner_secret;
     welcome_secret = bytes_to_hex_string welcome_secret;
     init_secret = bytes_to_hex_string init_secret;
