fstar/api/MLS.fst
@@ -696,7 +696,7 @@ let process_welcome_message w (sign_pk, sign_sk) lookup =
   let? interim_transcript_hash = MLS.TreeDEM.Message.Transcript.compute_interim_transcript_hash #bytes group_info.tbs.confirmation_tag group_info.tbs.group_context.confirmed_transcript_hash in
   let? tree_hash = MLS.TreeSync.API.compute_tree_hash treesync_state in
   let? group_context = compute_group_context group_info.tbs.group_context.group_id group_info.tbs.group_context.epoch tree_hash group_info.tbs.group_context.confirmed_transcript_hash in
-  let? epoch_secret = MLS.TreeKEM.KeySchedule.secret_joiner_to_epoch (secrets.joiner_secret <: bytes) [] (serialize _ group_context) in
+  let? epoch_secret = MLS.TreeKEM.KeySchedule.secret_joiner_to_epoch (secrets.joiner_secret <: bytes) [] group_context in
   let? (treekem_state, encryption_secret) = MLS.TreeKEM.API.welcome treekem leaf_decryption_key opt_path_secret_and_inviter_ind leaf_index epoch_secret in
 
   let? tree_hash = MLS.TreeSync.API.compute_tree_hash treesync_state in
